dist/gcc-compatible/lib/Hacl_Hash_Blake2s_bindings.ml
@@ -5,9 +5,6 @@ module Bindings(F:Cstubs.FOREIGN) =
     module Hacl_Streaming_Types_applied =
       (Hacl_Streaming_Types_bindings.Bindings)(Hacl_Streaming_Types_stubs)
     open Hacl_Streaming_Types_applied
-    module Hacl_Hash_Blake2b_applied =
-      (Hacl_Hash_Blake2b_bindings.Bindings)(Hacl_Hash_Blake2b_stubs)
-    open Hacl_Hash_Blake2b_applied
     let hacl_Hash_Blake2s_init =
       foreign "Hacl_Hash_Blake2s_init"
         ((ptr uint32_t) @-> (uint32_t @-> (uint32_t @-> (returning void))))
@@ -66,10 +63,13 @@ module Bindings(F:Cstubs.FOREIGN) =
     let hacl_Hash_Blake2s_malloc =
       foreign "Hacl_Hash_Blake2s_malloc"
         (void @-> (returning (ptr hacl_Hash_Blake2s_state_t)))
+    let hacl_Hash_Blake2s_reset_with_key =
+      foreign "Hacl_Hash_Blake2s_reset_with_key"
+        ((ptr hacl_Hash_Blake2s_state_t) @->
+           (ocaml_bytes @-> (uint32_t @-> (returning void))))
     let hacl_Hash_Blake2s_reset =
       foreign "Hacl_Hash_Blake2s_reset"
-        ((ptr hacl_Hash_Blake2s_state_t) @->
-           (k___uint32_t__uint8_t_ @-> (returning void)))
+        ((ptr hacl_Hash_Blake2s_state_t) @-> (returning void))
     let hacl_Hash_Blake2s_update =
       foreign "Hacl_Hash_Blake2s_update"
         ((ptr hacl_Hash_Blake2s_state_t) @->
